spot/GC.SPOT.HeapExpansion.fst
@@ -1684,6 +1684,34 @@ let spot_chunked_cheney_promote_head_split_preserves_old_non_blue_header
   CheneyPreservation.chunked_cheney_promote_head_split_preserves_old_non_blue_header
     minor major fp roots alloc_fuel src hdr
 
+let spot_chunked_cheney_promote_head_split_preserves_old_non_blue_field
+  (minor: minor_state) (major: MH.major_heap) (fp: U64.t)
+  (roots: Seq.seq U64.t) (alloc_fuel: nat) (src: obj_addr) (hdr: U64.t)
+  (j: nat) (field_addr: hp_addr) (old: U64.t)
+  : Lemma
+      (requires
+        alloc_fuel > 1 /\
+        GenInv.chunked_major_alloc_shape major fp alloc_fuel /\
+        SpecMajorAlloc.major_fl_chain_terminates
+          major fp alloc_fuel = true /\
+        GenInv.chunked_chain_objects_blue major fp alloc_fuel /\
+        CheneyPreservation.chunked_cheney_promote_split_ready
+          minor major fp roots alloc_fuel /\
+        Seq.mem src (MH.major_objects major) /\
+        MH.read_word_in_major major (hd_address src) == Some hdr /\
+        Obj.getColor hdr <> GC.Lib.Header.Blue /\
+        j < U64.v (Obj.getWosize hdr) /\
+        U64.v field_addr == U64.v src + j * U64.v mword /\
+        MH.read_word_in_major major field_addr == Some old)
+      (ensures
+        (let res =
+           ChunkedCheney.chunked_cheney_promote
+             minor major fp roots alloc_fuel in
+         MH.read_word_in_major res.major_final field_addr == Some old))
+  =
+  CheneyPreservation.chunked_cheney_promote_head_split_preserves_old_non_blue_field
+    minor major fp roots alloc_fuel src hdr j field_addr old
+
 let spot_chunked_cheney_promote_head_split_preserves_chain_objects_blue
   (minor: minor_state) (major: MH.major_heap) (fp: U64.t)
   (roots: Seq.seq U64.t) (alloc_fuel: nat)
